\documentclass{article}

\usepackage{amsfonts}
\usepackage{amsmath}
\usepackage{mathrsfs}

\usepackage{tikz}
\usetikzlibrary{quotes, angles, intersections}
\newcommand{\R}{\mathbb{R}}
\newcommand{\D}{\mathscr{D}}
\newcommand{\Pp}{\mathscr{P}}
\newcommand{\Cc}{\mathscr{C}}
\newcommand{\E}{\mathscr{E}}

\newcommand{\bigO}{\mathscr{O}}
%\usetikzlibrary{matrix}
%\usepackage{pgfplots}
%\pgfplotsset{compat=1.4}
\usepackage{algorithm2e}
\usepackage{algorithmic}

\usepackage{caption}
\newcommand{\source}[1]{\caption*{Source: {#1}} }

\begin{document}
	\section{Intro}
	
	\begin{align*}
	A(x_1^2-x_2^2) + B(x_1y_1-x_2y_2) + C(y_1^2-y_2^2) + D(x_1-x_2)+E(y_1-y_2) = 0\\
	A(x_1^2-x_3^2) + B(x_1y_1-x_3y_3) + C(y_1^2-y_3^2) + D(x_1-x_3)+E(y_1-y_3) = 0\\
	A(x_2^2-x_3^2) + B(x_2y_2-x_3y_3) + C(y_2^2-y_3^2) + D(x_2-x_3)+E(y_2-y_3) = 0\\
	\end{align*}
	
	From them we get:
	
	\begin{align*}
	D = -\frac{A(x_1^2-x_2^2) + B(x_1y_1-x_2y_2) + C(y_1^2-y_2^2) + E(y_1-y_2)}{x_1-x_2}\\
	E = -\frac{	A(x_1^2-x_3^2) + B(x_1y_1-x_3y_3) + C(y_1^2-y_3^2) + D(x_1-x_3)}{y_1-y_3}
	\end{align*}
	
	Inserting $E$ into $D$:
	
	\begin{align*}
	D(x_1-x_2) = -A(x_1^2-x_2^2) - B(x_1y_1-x_2y_2) - C(y_1^2-y_2^2) +\\
	\frac{	A(x_1^2-x_3^2) + B(x_1y_1-x_3y_3) + C(y_1^2-y_3^2) + D(x_1-x_3)}{y_1-y_3}(y_1-y_2)\\
	D(x_1-x_2 - \frac{(y_1-y_2)(x_1-x_3)}{y_1-y_3})=\\
	A(\frac{x_1^2-x_3^2}{y_1-y_3}-x_1^2+x_2^2)+\\
	B(\frac{x_1y_1-x_3y_3}{y_1-y_3} - x_1y_1 + x_2y_2)+\\
	C(\frac{y_1^2-y_3^2}{y_1-y_3}-y_1^2+y_2^2)
	\end{align*}
	
	Renaming things:
	
	\begin{align*}
	\alpha_d = x_1-x_2 -\frac{(x_1-x_3)(y_1-y_2)}{y_1-y_3}\\
	\alpha_a = \frac{x_1^2-x_3^2}{y_1-y_3}-x_1^2+x_2^2\\
	\alpha_b = \frac{x_1y_1-x_3y_3}{y_1-y_3} - x_1y_1 + x_2y_2\\
	\alpha_c = \frac{y_1^2-y_3^2}{y_1-y_3}-y_1^2+y_2^2\\
	D\alpha_d = A\alpha_a + B\alpha_b + C\alpha_c\\
	D=\frac{A\alpha_a + B\alpha_b + C\alpha_c}{\alpha_d}
	\end{align*}
	
	Going back to $(E)$:
	
	\begin{align*}
	E(y_1-y_3) = -A(x_1^2-x_3^2 - (x_1-x_3)\frac{\alpha_a}{\alpha_d}) - B(x_1y_1-x_3y_3 - (x_1-x_3)\frac{\alpha_b}{\alpha_d}) -C(y_1^2-y_3^2-(x_1-x_3)\frac{\alpha_c}{\alpha_d})
	\end{align*}
	
	Renaming things:
	
	\begin{align*}
	\beta_e = y_1-y_3\\
	\beta_a = -x_1^2+x_3^2 + (x_1-x_3)\frac{\alpha_a}{\alpha_d}\\
	\beta_b = -x_1y_1+x_3y_3 + (x_1-x_3)\frac{\alpha_b}{\alpha_d}\\
	\beta_c = -y_1^2+y_3^2+(x_1-x_3)\frac{\alpha_c}{\alpha_d}\\
	E\beta_e = A\beta_a + B\beta_b + C\beta_c\\
	E = \frac{A\beta_a + B\beta_b + C\beta_c}{\beta_e}
	\end{align*}
	
	Using the third equation:
	
	\begin{align*}
	A(x_2^2-x_3^2) + B(x_2y_2-x_3y_3) + C(y_2^2-y_3^2) +\\
	\frac{A\alpha_a + B\alpha_b + C\alpha_c}{\alpha_d}(x_2-x_3)+\\
	\frac{A\beta_a + B\beta_b + C\beta_c}{\beta_e}(y_2-y_3) = 0
	\end{align*}
	
	Now, isolating $B$:
	
	\begin{align*}
	A(x_2^2-x_3^2 + (x_2-x_3)\frac{\alpha_a}{\alpha_d} + (y_2-y_3)\frac{\beta_a}{\beta_e})+\\
	B(x_2y_2 -x_3y_3 + (x_2-x_3)\frac{\alpha_b}{\alpha_d} + (y_2-y_3)\frac{\beta_b}{\beta_e})+\\
	C(y_2^2-y_3^2 + (x_2-x_3)\frac{\alpha_c}{\alpha_d} + (y_2-y_3)\frac{\beta_c}{\beta_e})=0
	\end{align*}
	
	\begin{align*}
	\gamma_a = x_2^2-x_3^2 + (x_2-x_3)\frac{\alpha_a}{\alpha_d} + (y_2-y_3)\frac{\beta_a}{\beta_e}\\
	\gamma_b = (x_2y_2 -x_3y_3 + (x_2-x_3)\frac{\alpha_b}{\alpha_d} + (y_2-y_3)\frac{\beta_b}{\beta_e}\\
	\gamma_c = y_2^2-y_3^2 + (x_2-x_3)\frac{\alpha_c}{\alpha_d} + (y_2-y_3)\frac{\beta_c}{\beta_e}\\
	A\gamma_a + B\gamma_b + C\gamma_c = 0\\
	B = -\frac{A\gamma_a + C\gamma_c}{\gamma_b}
	\end{align*}
\end{document}